MLIR/Util/Tactics.lean
@@ -1,0 +1,11 @@
+
+-- TODO: I would hope that some tactic is already available for this?
+-- TODO: I don't know how to execute some tactics only in first goal, and some in second goal
+-- TODO: How can we have arbitrary terms instead of idents? term do not work
+
+/- `byCases H: x = y` splits the goal into one goal that has `x = y`, and one that hase `x ≠ y`.
+ `H` will contain the new hypothesis, and in the equality case, `x` will be substituted by `y`,
+ or `y` by `x` depending on which one will work.
+ `simp [H]` will be called on both subgoals. -/
+macro "byCases" Hname:ident ":" lhs:ident "=" rhs:ident : tactic =>   
+  `(tactic| apply Decidable.byCases (p:= $lhs = $rhs) <;> (intros $Hname) <;> (simp [$Hname:ident]) <;> (try subst $lhs) <;> (try subst $rhs))
